Valaig/Aig/GetSet.lean
@@ -34,27 +34,28 @@ LatchIdx.setNext Lemmas.
 section setNext
 variable {setIdx : LatchIdx} {setValid : setIdx.validIn aig} {newNext : Lit}
 
-@[simp, grind =>]
+@[simp, grind =]
 theorem get_LatchIdx_setNext {var : Var} {valid : var.validIn aig} :
     (setIdx.setNext aig newNext setValid).get var = aig.get var valid := by
   simp
 
+@[simp, grind =]
 theorem InputIdx.getVar_LatchIdx_setNext {idx : InputIdx} {valid : idx.validIn aig} :
     idx.getVar (setIdx.setNext aig newNext setValid) = idx.getVar aig := by
   simp
 
-@[simp, grind =>]
+@[simp, grind =]
 theorem LatchIdx.getVar_LatchIdx_setNext {idx : LatchIdx} {valid : idx.validIn aig} :
     idx.getVar (setIdx.setNext aig newNext setValid) = idx.getVar aig := by
   simp; grind
 
-@[simp, grind =>]
-theorem LatchIdx.getNext_LatchIdx_setNext {idx : LatchIdx} {valid : idx.validIn aig} :
+@[simp, grind =]
+theorem LatchIdx.getNext_LatchIdx_setNext_self {idx : LatchIdx} {valid : idx.validIn aig} :
     idx.getNext (setIdx.setNext aig newNext setValid) =
     if idx = setIdx then newNext else idx.getNext aig := by
   simp; grind
 
-@[simp, grind =>]
+@[simp, grind =]
 theorem LatchIdx.getReset_LatchIdx_setNext {idx : LatchIdx} {valid : idx.validIn aig} :
     idx.getReset (setIdx.setNext aig newNext setValid) = idx.getReset aig := by
   simp; grind
@@ -67,26 +68,27 @@ LatchIdx.setReset Lemmas.
 section setReset
 variable {setIdx : LatchIdx} {setValid : setIdx.validIn aig} {newReset : Lit}
 
-@[simp, grind =>]
+@[simp, grind =]
 theorem get_LatchIdx_setReset {var : Var} {valid : var.validIn aig} :
     (setIdx.setReset aig newReset setValid).get var = aig.get var valid := by
   simp
 
+@[simp, grind =]
 theorem InputIdx.getVar_LatchIdx_setReset {idx : InputIdx} {valid : idx.validIn aig} :
     idx.getVar (setIdx.setReset aig newReset setValid) = idx.getVar aig := by
   simp
 
-@[simp, grind =>]
+@[simp, grind =]
 theorem LatchIdx.getVar_LatchIdx_setReset {idx : LatchIdx} {valid : idx.validIn aig} :
     idx.getVar (setIdx.setReset aig newReset setValid) = idx.getVar aig := by
   simp; grind
 
-@[simp, grind =>]
+@[simp, grind =]
 theorem LatchIdx.getNext_LatchIdx_setReset {idx : LatchIdx} {valid : idx.validIn aig} :
     idx.getNext (setIdx.setReset aig newReset setValid) = idx.getNext aig := by
   simp; grind
 
-@[simp, grind =>]
+@[simp, grind =]
 theorem LatchIdx.getReset_LatchIdx_setReset {idx : LatchIdx} {valid : idx.validIn aig} :
     idx.getReset (setIdx.setReset aig newReset setValid) =
     if idx = setIdx then newReset else idx.getReset aig := by
@@ -104,27 +106,27 @@ Aig.addInput Lemmas.
 -/
 section addInput
 
-@[simp, grind =>]
+@[simp, grind =]
 theorem get_Aig_addInput {var : Var} {valid : var.validIn aig} :
     aig.addInput.fst.get var = aig.get var valid := by
   simp; grind
 
-@[simp, grind =>]
+@[simp, grind =]
 theorem InputIdx.getVar_Aig_addInput {idx : InputIdx} {valid : idx.validIn aig} :
     idx.getVar aig.addInput.fst = idx.getVar aig valid := by
   simp; grind
 
-@[simp, grind =>]
+@[simp, grind =]
 theorem LatchIdx.getVar_Aig_addInput {idx : LatchIdx} {valid : idx.validIn aig} :
     idx.getVar aig.addInput.fst = idx.getVar aig valid := by
   simp
 
-@[simp, grind =>]
+@[simp, grind =]
 theorem LatchIdx.getNext_Aig_addInput {idx : LatchIdx} {valid : idx.validIn aig} :
     idx.getNext aig.addInput.fst = idx.getNext aig valid := by
   simp
 
-@[simp, grind =>]
+@[simp, grind =]
 theorem LatchIdx.getReset_Aig_addInput {idx : LatchIdx} {valid : idx.validIn aig} :
     idx.getReset aig.addInput.fst = idx.getReset aig valid := by
   simp
@@ -137,22 +139,22 @@ Aig.addLatch Lemmas.
 section addLatch
 variable {next reset : Lit}
 
-@[simp, grind =>]
+@[simp, grind =]
 theorem get_Aig_addLatch {var : Var} {valid : var.validIn aig} :
     (aig.addLatch next reset).fst.get var = aig.get var valid := by
   simp; grind
 
-@[simp, grind =>]
+@[simp, grind =]
 theorem InputIdx.getVar_Aig_addLatch {idx : InputIdx} {valid : idx.validIn aig} :
     idx.getVar (aig.addLatch next reset).fst = idx.getVar aig valid := by
   simp
 
-@[simp, grind =>]
+@[simp, grind =]
 theorem LatchIdx.getVar_Aig_addLatch {idx : LatchIdx} {valid : idx.validIn aig} :
     idx.getVar (aig.addLatch next reset).fst = idx.getVar aig valid := by
   simp; grind
 
-@[simp, grind =>]
+@[simp, grind =]
 theorem LatchIdx.getNext_Aig_addLatch {idx : LatchIdx} {valid : idx.validIn aig} :
     idx.getNext (aig.addLatch next reset).fst = idx.getNext aig valid := by
   simp; grind
@@ -162,7 +164,7 @@ theorem LatchIdx.getNext_Aig_addLatch_eq_self :
   (aig.addLatch next reset).snd.getNext (aig.addLatch next reset).fst = next := by
   simp
 
-@[simp, grind =>]
+@[simp, grind =]
 theorem LatchIdx.getReset_Aig_addLatch {idx : LatchIdx} {valid : idx.validIn aig} :
     idx.getReset (aig.addLatch next reset).fst = idx.getReset aig valid := by
   simp; grind
@@ -180,27 +182,27 @@ Aig.addAnd Lemmas.
 section addAnd
 variable {rhs0 rhs1 : Lit} {h0 : rhs0.validIn aig} {h1 : rhs1.validIn aig}
 
-@[simp, grind =>]
+@[simp, grind =]
 theorem get_Aig_addAnd {var : Var} {valid : var.validIn aig} :
     (aig.addAnd rhs0 rhs1 h0 h1).fst.get var = aig.get var valid := by
   simp; grind
 
-@[simp, grind =>]
+@[simp, grind =]
 theorem InputIdx.getVar_Aig_addAnd {idx : InputIdx} {valid : idx.validIn aig} :
     idx.getVar (aig.addAnd rhs0 rhs1 h0 h1).fst = idx.getVar aig valid := by
   simp
 
-@[simp, grind =>]
+@[simp, grind =]
 theorem LatchIdx.getVar_Aig_addAnd {idx : LatchIdx} {valid : idx.validIn aig} :
     idx.getVar (aig.addAnd rhs0 rhs1 h0 h1).fst = idx.getVar aig valid := by
   simp
 
-@[simp, grind =>]
-theorem LatchIdx.getNext_Aig_addAnd {idx : LatchIdx} {valid : idx.validIn aig} :
+@[simp, grind =]
+theorem LatchId.getNext_Aig_addAnd {idx : LatchIdx} {valid : idx.validIn aig} :
     idx.getNext (aig.addAnd rhs0 rhs1 h0 h1).fst = idx.getNext aig valid := by
   simp
 
-@[simp, grind =>]
+@[simp, grind =]
 theorem LatchIdx.getReset_Aig_addAnd {idx : LatchIdx} {valid : idx.validIn aig} :
     idx.getReset (aig.addAnd rhs0 rhs1 h0 h1).fst = idx.getReset aig valid := by
   simp
