Valaig/Aig/IdxValidity.lean
@@ -25,12 +25,12 @@ section latch
 variable {latch : LatchIdx} {valid : latch.validIn aig}
 
 @[simp, grind =]
-theorem LatchIdx.setNext_genericIdx_mono {next : Lit} (idx : GenericIdx) :
+theorem LatchIdx.validIn_setNext {next : Lit} (idx : GenericIdx) :
     idx.validIn (setNext latch aig next valid) ↔ idx.validIn aig := by
   simp
 
 @[simp, grind =]
-theorem LatchIdx.setReset_genericIdx_mono {reset : Lit} (idx : GenericIdx) :
+theorem LatchIdx.validIn_setReset {reset : Lit} (idx : GenericIdx) :
     idx.validIn (setReset latch aig reset valid) ↔ idx.validIn aig := by
   simp
 
@@ -42,22 +42,22 @@ section atom
 addInput Lemmas.
 -/
 
-@[grind .]
-theorem addInput_genericIdx_mono_impl (idx : GenericIdx) :
+theorem validIn_addInput (idx : GenericIdx) :
     idx.validIn aig → idx.validIn aig.addInput.fst := by
   simp; grind only
 
-@[simp, grind =]
-theorem addInput_genericIdx_mono (idx : GenericIdx) :
-    idx.validIn aig.addInput.fst ↔
-    (idx.validIn aig
-    ∨ idx = .input aig.addInput.snd
-    ∨ idx = .node (aig.addInput.snd.getVar aig.addInput.fst)) := by
-  simp; grind
+grind_pattern validIn_addInput => idx.validIn aig.addInput.fst where
+  idx =/= .input aig.addInput.snd
+  idx =/= .node (aig.addInput.snd.getVar aig.addInput.fst)
 
-@[grind .]
-theorem addInput_self_validIn :
+@[simp, grind .]
+theorem addInput_validIn :
     aig.addInput.snd.validIn aig.addInput.fst := by
+  simp
+
+@[simp, grind .]
+theorem addInput_getVar_validIn :
+    (aig.addInput.snd.getVar aig.addInput.fst).validIn aig.addInput.fst := by
   simp
 
 /-
@@ -66,22 +66,23 @@ addLatch Lemmas.
 section latch
 variable {next reset : Lit}
 
-@[grind .]
-theorem addLatch_genericIdx_mono_impl (idx : GenericIdx) :
+theorem validIn_addLatch (idx : GenericIdx) :
     idx.validIn aig → idx.validIn (aig.addLatch next reset).fst := by
   simp; grind only
 
-@[simp, grind =]
-theorem addLatch_genericIdx_mono (idx : GenericIdx) :
-    idx.validIn (aig.addLatch next reset).fst ↔
-    (idx.validIn aig
-    ∨ idx = .latch (aig.addLatch next reset).snd
-    ∨ idx = .node ((aig.addLatch next reset).snd.getVar (aig.addLatch next reset).fst)) := by
-  simp; grind
+grind_pattern validIn_addLatch => idx.validIn (aig.addLatch next reset).fst where
+  idx =/= .latch (aig.addLatch next reset).snd
+  idx =/= .node ((aig.addLatch next reset).snd.getVar (aig.addLatch next reset).fst)
 
-@[grind .]
-theorem addLatch_self_validIn :
+@[simp, grind .]
+theorem addLatch_validIn :
     (aig.addLatch next reset).snd.validIn (aig.addLatch next reset).fst := by
+  simp
+
+@[simp, grind .]
+theorem addLatch_getVar_validIn :
+    (aig.addLatch next reset).snd.getVar (aig.addLatch next reset).fst |>.validIn
+      (aig.addLatch next reset).fst := by
   simp
 
 end latch
@@ -93,16 +94,17 @@ addAnd Lemmas.
 section gate
 variable {rhs0 rhs1 : Lit} {h0 : rhs0.validIn aig} {h1 : rhs1.validIn aig}
 
-@[grind .]
-theorem addAnd_genericIdx_mono_impl (idx : GenericIdx) :
+theorem validIn_addAnd (idx : GenericIdx) :
     idx.validIn aig → idx.validIn (aig.addAnd rhs0 rhs1 h0 h1).fst := by
   simp; grind
 
-@[grind .]
-theorem addAnd_self_validIn :
+grind_pattern validIn_addAnd => idx.validIn (aig.addAnd rhs0 rhs1 h0 h1).fst where
+  idx =/= .node (aig.addAnd rhs0 rhs1 h0 h1).snd.var
+
+@[simp, grind .]
+theorem addAnd_validIn :
     (aig.addAnd rhs0 rhs1 h0 h1).snd.validIn (aig.addAnd rhs0 rhs1 h0 h1).fst := by
   simp
-  -- TODO: Whycan't I get grind to see this another way
   have {aig : Std.Sat.AIG AtomIdx} {entry: aig.Ref} := entry.hgate
   grind only
 
